wip: functional correctness for crypto_kem_decaps

frodo/code/Hacl.Impl.Frodo.KEM.Decaps.fst
@@ -37,9 +37,11 @@ val frodo_sub_mul_c_minus_bs_inner:
   -> mu_decode:lbytes (params_nbar *! params_nbar *! params_extracted_bits /. size 8)
   -> Stack unit
     (requires fun h ->
-      live h s_matrix /\ live h bp_matrix /\ 
+      live h s_matrix /\ live h bp_matrix /\
       live h c_matrix /\ live h mu_decode)
-    (ensures fun h0 _ h1 -> modifies (loc_buffer mu_decode) h0 h1)
+    (ensures fun h0 _ h1 -> modifies (loc_buffer mu_decode) h0 h1 /\
+      (let m_matrix = M.sub (as_matrix h0 c_matrix) (M.mul_s (as_matrix h0 bp_matrix) (as_matrix h0 s_matrix)) in
+       as_seq h1 mu_decode == Spec.Frodo.Encode.frodo_key_decode (v params_extracted_bits) m_matrix))
 let frodo_sub_mul_c_minus_bs_inner s_matrix bp_matrix c_matrix mu_decode =
   push_frame();
   let m_matrix = matrix_create params_nbar params_nbar in
@@ -56,7 +58,8 @@ val frodo_sub_mul_c_minus_bs:
   -> Stack unit
     (requires fun h ->
       live h sk /\ live h bp_matrix /\ live h c_matrix /\ live h mu_decode)
-    (ensures fun h0 r h1 -> modifies (loc_buffer mu_decode) h0 h1)
+    (ensures fun h0 _ h1 -> modifies (loc_buffer mu_decode) h0 h1 /\
+      as_seq h1 mu_decode == S.frodo_sub_mul_c_minus_bs (as_seq h0 sk) (as_matrix h0 bp_matrix) (as_matrix h0 c_matrix))
 [@"c_inline"]
 let frodo_sub_mul_c_minus_bs sk bp_matrix c_matrix mu_decode =
   push_frame();
@@ -76,31 +79,25 @@ val get_dec_ss:
     (requires fun h ->
       live h ct /\ live h kp_s /\ live h ss /\
       disjoint ss ct /\ disjoint ss kp_s)
-    (ensures fun h0 r h1 -> modifies (loc_buffer ss) h0 h1)
+    (ensures fun h0 _ h1 -> modifies (loc_buffer ss) h0 h1 /\
+      as_seq h1 ss == S.get_dec_ss (as_seq h0 ct) (as_seq h0 kp_s))
 let get_dec_ss ct kp_s ss =
   push_frame();
-  Spec.Frodo.KEM.expand_crypto_ciphertextbytes ();
-  let c1Len = params_logq *! params_nbar *! params_n /. size 8 in
-  let c2Len = params_logq *! params_nbar *! params_nbar /. size 8 in
-  let c12 = sub #uint8 #_ #(v c1Len + v c2Len) ct (size 0) (c1Len +! c2Len) in
-  let d = sub #uint8 #_ #(v crypto_bytes) ct (c1Len +! c2Len) crypto_bytes in
+  let c12 = sub ct (size 0) (crypto_ciphertextbytes -! crypto_bytes) in
+  let d = sub #uint8 #_ #(v crypto_bytes) ct (crypto_ciphertextbytes -! crypto_bytes) crypto_bytes in
 
-  let ss_init_len = c1Len +! c2Len +! size 2 *! crypto_bytes in
+  let ss_init_len = crypto_ciphertextbytes +! crypto_bytes in
   let ss_init:lbytes ss_init_len = create ss_init_len (u8 0) in
-  update_sub ss_init (size 0) (c1Len +! c2Len) c12;
-  update_sub ss_init (c1Len +! c2Len) crypto_bytes kp_s;
-  update_sub ss_init (ss_init_len -! crypto_bytes) crypto_bytes d;
+  update_sub ss_init (size 0) (crypto_ciphertextbytes -! crypto_bytes) c12;
+  update_sub ss_init (crypto_ciphertextbytes -! crypto_bytes) crypto_bytes kp_s;
+  update_sub ss_init crypto_ciphertextbytes crypto_bytes d;
 
   cshake_frodo ss_init_len ss_init (u16 7) crypto_bytes ss;
   pop_frame()
 
-let pk_mu_decode_len =
-  assert_norm (v crypto_publickeybytes + v params_nbar * v params_nbar * v params_extracted_bits / 8 < max_size_t);
-  normalize_term (crypto_publickeybytes +! params_nbar *! params_nbar *! params_extracted_bits /. size 8)
-
 inline_for_extraction noextract
 val get_bpp_cp_matrices:
-    g:lbytes (size 3 *! crypto_bytes)
+     g:lbytes (size 3 *! crypto_bytes)
   -> mu_decode:lbytes (params_nbar *! params_nbar *! params_extracted_bits /. size 8)
   -> sk:lbytes crypto_secretkeybytes
   -> bpp_matrix:matrix_t params_nbar params_n
@@ -112,9 +109,11 @@ val get_bpp_cp_matrices:
       disjoint g bpp_matrix /\ disjoint sk bpp_matrix /\
       disjoint mu_decode bpp_matrix /\ disjoint mu_decode cp_matrix /\
       disjoint g cp_matrix /\ disjoint sk cp_matrix /\ disjoint bpp_matrix cp_matrix)
-    (ensures fun h0 _ h1 -> modifies (loc_union (loc_buffer bpp_matrix) (loc_buffer cp_matrix)) h0 h1)
-let get_bpp_cp_matrices g mu_decode sk bpp_matrix cp_matrix  =
-  assert_norm (v params_nbar * v params_n % 2 = 0);
+    (ensures fun h0 _ h1 -> modifies (loc_union (loc_buffer bpp_matrix) (loc_buffer cp_matrix)) h0 h1 /\
+      (let bpp_matrix_sp, cp_matrix_sp = S.get_bpp_cp_matrices (as_seq h0 g) (as_seq h0 mu_decode) (as_seq h0 sk) in
+       as_matrix h1 bpp_matrix == bpp_matrix_sp /\ as_matrix h1 cp_matrix == cp_matrix_sp))
+let get_bpp_cp_matrices g mu_decode sk bpp_matrix cp_matrix =
+  assert (v params_nbar * v params_n % 2 = 0);
   push_frame();
   Spec.Frodo.KEM.expand_crypto_publickeybytes ();
   Spec.Frodo.KEM.expand_crypto_secretkeybytes ();
@@ -146,24 +145,29 @@ val crypto_kem_dec_ss_inner:
       live h c_matrix /\ live h sk /\ live h ct /\ live h ss /\
       disjoint ss ct /\ disjoint ss sk /\ disjoint ss mu_decode /\
       disjoint ss bp_matrix /\ disjoint ss c_matrix /\ disjoint ss g)
-    (ensures fun h0 _ h1 -> modifies (loc_buffer ss) h0 h1)
-let crypto_kem_dec_ss_inner mu_decode g bp_matrix c_matrix sk ct ss =
+    (ensures fun h0 _ h1 -> modifies (loc_buffer ss) h0 h1 /\
+      as_seq h1 ss == S.crypto_kem_dec_ss_inner (as_seq h0 mu_decode) (as_seq h0 g)
+      (as_matrix h0 bp_matrix) (as_matrix h0 c_matrix) (as_seq h0 sk) (as_seq h0 ct))
+let crypto_kem_dec_ss_inner mu_decode g bp_matrix c_matrix sk ct ss = admit();
   push_frame();
   Spec.Frodo.KEM.expand_crypto_ciphertextbytes ();
   Spec.Frodo.KEM.expand_crypto_secretkeybytes ();
-
-  let bpp_matrix = matrix_create params_nbar params_n in
-  let cp_matrix  = matrix_create params_nbar params_nbar in
-  get_bpp_cp_matrices g mu_decode sk bpp_matrix cp_matrix;
 
   let dp = sub #uint8 #_ #(v crypto_bytes) g (size 2 *! crypto_bytes) crypto_bytes in
   let d = sub #uint8 #_ #(v crypto_bytes) ct (crypto_ciphertextbytes -! crypto_bytes) crypto_bytes in
   let kp = sub #uint8 #_ #(v crypto_bytes) g crypto_bytes crypto_bytes in
   let s = sub #uint8 #_ #(v crypto_bytes) sk (size 0) crypto_bytes in
-
+ 
+  let bpp_matrix = matrix_create params_nbar params_n in
+  let cp_matrix  = matrix_create params_nbar params_nbar in
+  let h0 = ST.get () in
+  get_bpp_cp_matrices g mu_decode sk bpp_matrix cp_matrix;
   let b1 = lbytes_eq d dp in
+  //assume (b1 == Lib.Sequence.lbytes_eq #(v crypto_bytes) (as_seq h0 d) (as_seq h0 dp));
   let b2 = matrix_eq params_logq bp_matrix bpp_matrix in
+  assert (b2 == M.matrix_eq (v params_logq) (as_matrix h0 bp_matrix) (as_matrix h0 bpp_matrix));
   let b3 = matrix_eq params_logq c_matrix cp_matrix in
+  assert (b3 == M.matrix_eq (v params_logq) (as_matrix h0 c_matrix) (as_matrix h0 cp_matrix));
   let kp_s = if (b1 && b2 && b3) then kp else s in
   get_dec_ss ct kp_s ss;
   pop_frame()
@@ -183,12 +187,13 @@ val crypto_kem_dec_ss:
       disjoint ss bp_matrix /\ disjoint ss c_matrix)
     (ensures fun h0 _ h1 -> modifies (loc_buffer ss) h0 h1)
 [@"c_inline"]
-let crypto_kem_dec_ss mu_decode bp_matrix c_matrix sk ct ss =
-  push_frame();
+let crypto_kem_dec_ss mu_decode bp_matrix c_matrix sk ct ss = admit();
+  let mu_decode_len = params_nbar *! params_nbar *! params_extracted_bits /. size 8 in
+  let pk_mu_decode_len = crypto_publickeybytes +! mu_decode_len in
   assert_norm (v pk_mu_decode_len =
     v crypto_publickeybytes + v params_nbar * v params_nbar * v params_extracted_bits / 8);
 
-  let mu_decode_len = params_nbar *! params_nbar *! params_extracted_bits /. size 8 in
+  push_frame();
   let pk_mu_decode = create pk_mu_decode_len (u8 0) in
   let pk = sub #uint8 #_ #(v crypto_publickeybytes) sk crypto_bytes crypto_publickeybytes in
   update_sub pk_mu_decode (size 0) crypto_publickeybytes pk;
